lib/Base/Multisets.i.dfy
@@ -1,0 +1,173 @@
+module Multisets {
+  function {:opaque} Choose<A>(s: multiset<A>) : (result: A)
+    requires 0 < |s|
+    ensures result in s
+  {
+    var a :| a in s;
+    a
+  }
+
+  function {:opaque} Apply<A, B>(fn: A ~> B, s: multiset<A>) : (result: multiset<B>)
+    requires forall x | x in s :: fn.requires(x)
+    ensures |s| == 0 ==> |result| == 0
+    reads set x, o | x in s && o in fn.reads(x) :: o
+  {
+    if |s| == 0 then
+      multiset{}
+    else
+      var x := Choose(s);
+      multiset{fn(x)} + Apply(fn, s - multiset{x})
+  }
+
+  lemma ApplySingleton<A, B>(fn: A ~> B, x: A)
+    requires fn.requires(x)
+    ensures Apply(fn, multiset{x}) == multiset{fn(x)}
+  {
+    reveal_Apply();
+  }
+  
+  lemma ApplyAdditive<A,B>(fn: A ~> B, s1: multiset<A>, s2: multiset<A>)
+    requires forall x | x in s1 :: fn.requires(x)
+    requires forall x | x in s2 :: fn.requires(x)
+    ensures Apply(fn, s1+s2) == Apply(fn, s1) + Apply(fn, s2)
+    decreases |s1| + |s2|
+  {
+    if |s1| == 0 {
+      assert s1 + s2 == s2;
+    } else if |s2| == 0 {
+      assert s1 + s2 == s1;
+    } else {
+      var x := Choose(s1 + s2);
+      if x in s1 {
+        calc {
+          Apply(fn, s1+s2);
+          { reveal_Apply(); }
+          multiset{fn(x)} + Apply(fn, (s1+s2) - multiset{x});
+          { assert (s1+s2) - multiset{x} == (s1 - multiset{x}) + s2; }
+          multiset{fn(x)} + Apply(fn, (s1 - multiset{x}) + s2);
+          { ApplyAdditive(fn, s1 - multiset{x}, s2); }
+          multiset{fn(x)} + Apply(fn, s1 - multiset{x}) + Apply(fn, s2);
+          { reveal_Apply(); }
+          Apply(fn, multiset{x}) + Apply(fn, s1 - multiset{x}) + Apply(fn, s2);
+          { ApplyAdditive(fn, multiset{x}, s1 - multiset{x}); }
+          Apply(fn, multiset{x} + (s1 - multiset{x})) + Apply(fn, s2);
+          { assert multiset{x} + (s1 - multiset{x}) == s1; }
+          Apply(fn, s1) + Apply(fn, s2);
+        }
+      } else {
+        calc {
+          Apply(fn, s1+s2);
+          { reveal_Apply(); }
+          multiset{fn(x)} + Apply(fn, (s1+s2) - multiset{x});
+          { assert (s1+s2) - multiset{x} == s1 + (s2 - multiset{x}); }
+          multiset{fn(x)} + Apply(fn, s1 + (s2 - multiset{x}));
+          { ApplyAdditive(fn, s1, s2 - multiset{x}); }
+          multiset{fn(x)} + Apply(fn, s1) + Apply(fn, s2 - multiset{x});
+          { reveal_Apply(); }
+          Apply(fn, multiset{x}) + Apply(fn, s1) + Apply(fn, s2 - multiset{x});
+          { ApplyAdditive(fn, multiset{x}, s2 - multiset{x}); }
+          Apply(fn, multiset{x} + (s2 - multiset{x})) + Apply(fn, s1);
+          { assert multiset{x} + (s2 - multiset{x}) == s2; }
+          Apply(fn, s1) + Apply(fn, s2);
+        }
+      }
+    }
+  }
+  
+  function {:opaque} Fold<A>(zero: A, add: (A, A) -> A, s: multiset<A>) : (result: A)
+    ensures |s| == 0 ==> result == zero
+  {
+    if |s| == 0 then
+      zero
+    else
+      var a := Choose(s);
+      add(a, Fold(zero, add, s - multiset{a}))
+  }
+
+  lemma FoldSingleton<A>(zero: A, add: (A, A) -> A, x: A)
+    ensures Fold(zero, add, multiset{x}) == add(x, zero)
+  {
+    reveal_Fold();
+  }
+  
+  predicate {:opaque} IsIdentity<A(!new)>(add: (A, A) -> A, zero: A) {
+    && forall a :: add(zero, a) == add(a, zero) == a
+  }
+
+  predicate {:opaque} IsCommutative<A(!new)>(add: (A, A) -> A) {
+    forall a, b :: add(a, b) == add(b, a)
+  }
+
+  predicate {:opaque} IsAssociative<A(!new)>(add: (A, A) -> A) {
+    forall a, b, c :: add(add(a, b), c) == add(a, add(b, c))
+  }
+
+  lemma FoldAdditive<A>(zero: A, add: (A, A) -> A, s1: multiset<A>, s2: multiset<A>)
+    requires IsCommutative(add)
+    requires IsAssociative(add)
+    requires IsIdentity(add, zero)
+    ensures Fold(zero, add, s1 + s2) == add(Fold(zero, add, s1), Fold(zero, add, s2))
+    decreases |s1| + |s2|
+  {
+    var f1 := Fold(zero, add, s1);
+    var f2 := Fold(zero, add, s2);
+    var fs := Fold(zero, add, s1 + s2);
+    if |s1| == 0 {
+      assert s1 + s2 == s2;
+      assert add(f1, f2) == Fold(zero, add, s2) by {
+        reveal_IsIdentity();
+        reveal_Fold();
+      }
+    } else if |s2| == 0 {
+      assert s1 + s2 == s1;
+      assert add(f1, f2) == Fold(zero, add, s1) by {
+        reveal_IsIdentity();
+        reveal_Fold();
+      }
+    } else {
+      var x := Choose(s1 + s2);
+      assert x in s1 || x in s2;
+      if x in s1 {
+        calc {
+          fs;
+          { reveal_Fold(); }
+          add(x, Fold(zero, add, (s1 + s2) - multiset{x}));
+          { assert (s1 + s2) - multiset{x} == (s1 - multiset{x}) + s2; }
+          add(x, Fold(zero, add, (s1 - multiset{x}) + s2));
+          { FoldAdditive(zero, add, s1 - multiset{x}, s2); }
+          add(x, add(Fold(zero, add, s1 - multiset{x}), Fold(zero, add, s2)));
+          { reveal_IsAssociative(); }
+          add(add(x, Fold(zero, add, s1 - multiset{x})), Fold(zero, add, s2));
+          { reveal_IsIdentity(); reveal_Fold(); }
+          add(add(Fold(zero, add, multiset{x}), Fold(zero, add, s1 - multiset{x})), Fold(zero, add, s2));
+          { FoldAdditive(zero, add, multiset{x}, s1 - multiset{x}); }
+          add(Fold(zero, add, multiset{x} + (s1 - multiset{x})), Fold(zero, add, s2));
+          { assert multiset{x} + (s1 - multiset{x}) == s1; }
+          add(Fold(zero, add, s1), Fold(zero, add, s2));
+        }
+      } else {
+        calc {
+          fs;
+          { reveal_Fold(); }
+          add(x, Fold(zero, add, (s1 + s2) - multiset{x}));
+          { assert (s1 + s2) - multiset{x} == s1 + (s2 - multiset{x}); }
+          add(x, Fold(zero, add, s1 + (s2 - multiset{x})));
+          { FoldAdditive(zero, add, s1, s2 - multiset{x}); }
+          add(x, add(Fold(zero, add, s1), Fold(zero, add, s2 - multiset{x})));
+          { reveal_IsAssociative(); }
+          add(add(x, Fold(zero, add, s1)), Fold(zero, add, s2 - multiset{x}));
+          { reveal_IsCommutative(); }
+          add(add(Fold(zero, add, s1), x), Fold(zero, add, s2 - multiset{x}));
+          { reveal_IsAssociative(); }
+          add(Fold(zero, add, s1), add(x, Fold(zero, add, s2 - multiset{x})));
+          { reveal_IsIdentity(); reveal_Fold(); }
+          add(Fold(zero, add, s1), add(Fold(zero, add, multiset{x}), Fold(zero, add, s2 - multiset{x})));
+          { FoldAdditive(zero, add, multiset{x}, s2 - multiset{x}); }
+          add(Fold(zero, add, s1), Fold(zero, add, multiset{x} + (s2 - multiset{x})));
+          assert multiset{x} + (s2 - multiset{x}) == s2;
+          add(Fold(zero, add, s1), Fold(zero, add, s2));
+        }
+      }
+    }
+  }
+}
